Fp/Multiplication.lean
@@ -1,0 +1,50 @@
+import Fp.Basic
+import Fp.Rounding
+
+def f_mul (a : FixedPoint v e) (b : FixedPoint w f) : FixedPoint (v+w) (e+f) :=
+  let hExOffset := Nat.add_lt_add a.hExOffset b.hExOffset
+  let a' : BitVec (v+w) := a.val.setWidth' (by omega)
+  let b' : BitVec (v+w) := b.val.setWidth' (by omega)
+  {
+    sign := a.sign ^^ b.sign
+    val := a' * b'
+    hExOffset
+  }
+
+def e_mul (a : EFixedPoint v e) (b : EFixedPoint w f) : EFixedPoint (v+w) (e+f) :=
+  let hExOffset := Nat.add_lt_add a.num.hExOffset b.num.hExOffset
+  open EFixedPoint in
+  if hN : a.state = .NaN || b.state = .NaN then getNaN hExOffset
+  else if hI1 : a.state = .Infinity || b.state = .Infinity then
+    getInfinity (a.num.sign ^^ b.num.sign) hExOffset
+  else
+    let _ : a.state = .Number && b.state = .Number := by
+      cases ha : a.state <;> cases hb : b.state <;> simp_all
+    {
+      state := .Number
+      num := f_mul a.num b.num
+    }
+
+def mul (he : 0 < e) (a b : PackedFloat e s) : PackedFloat e s :=
+  round _ _ (e_mul (a.toEFixed he) (b.toEFixed he))
+
+theorem FixedPoint_mul_comm (a b : FixedPoint 34 16)
+  : (f_mul a b) = (f_mul b a) := by
+  simp [f_mul]
+  bv_decide +acNf
+
+theorem EFixedPoint_mul_comm (a b : EFixedPoint 34 16)
+  : (e_mul a b) = (e_mul b a) := by
+  simp [e_mul]
+  cases ha2 : a.state <;> cases hb2 : b.state <;>
+    simp_all [Bool.xor_comm, FixedPoint_mul_comm]
+
+theorem EFixedPoint_mul_comm_brute (a b : EFixedPoint 4 2)
+  : (e_mul a b) = (e_mul b a) := by
+  apply EFixedPoint.inj
+  simp [e_mul, f_mul]
+  bv_decide +acNf
+
+theorem PackedFloat_mul_comm (a b : PackedFloat 5 2)
+  : (mul (by omega) a b) = (mul (by omega) b a) := by
+  simp [mul, EFixedPoint_mul_comm]
